# New Functions from Old Functions

## Transformations of Functions

***Vertical and Horizontal Shifts***

Suppose $c > 0$. To obtain the graph of

- $y = f(x) + c$, shift the graph of $y = f(x)$ a distance $c$ units upward
- $y = f(x) - c$, shift the graph of $y = f(x)$ a distance $c$ units downward
- $y = f(x - c)$, shift the graph of $y = f(x)$ a distance $c$ units to the right
- $y = f(x + c)$, shift the graph of $y = f(x)$ a distance $c$ units to the left

![](./img/1.11.png ':figure :size=50% Translating the graph of f.')

***Vertical and Horizontal Stretching and Reflecting***

Suppose $c > 1$. To obtain the graph of

- $y = cf(x)$, stretch the graph of $y = f(x)$ vertically by a factor of $c$
- $y = (\dfrac{1}{c})f(x)$, shrink the graph of $y = f(x)$ vertically by a factor of $c$
- $y = f(cx)$, shrink the graph of $y = f(x)$ horizontally by a factor of $c$
- $y = f(\dfrac{x}{c})$, stretch the graph of $y = f(x)$ horizontally by a factor of $c$
- $y = -f(x)$, reflect the graph of $y = f(x)$ about the x-axis
- $y = f(-x)$, reflect the graph of $y = f(x)$ about the y-axis

![](./img/1.12.png ':figure :size=50% Stretching and reflecting the graph of f.')

![](./img/1.13.png ':figure Stretching transformations.')

## Combinations of Functions

<div class="alert-note">

Given two functions $f$ and $g$, the *sum*, *difference*, *product*, and *quotient* functions are defined by

- $(f+g)(x) = f(x) + g(x)$
- $(f-g)(x) = f(x) - g(x)$
- $(fg)(x) = f(x) g(x)$
- $\Big( \dfrac{f}{g} \Big)(x) = \dfrac{f(x)}{g(x)}$

If the domain of $f$ is $A$ and the domain of $g$ is $B$, then:

- The domain of $f+g$ is $A \cap B$ because both $f(x)$ and $g(x)$ have to be defined.
- The domain of $f-g$ is also $A \cap B$.
- The domain of $fg$ is also $A \cap B$.
- Because we canâ€™t divide by 0, the domain of $\dfrac{f}{g}$ is $\{ x \in A \cap B \mid g(x) \neq 0 \}$

</div>

<div class="alert-note">

Given two functions $f$ and $g$, the **composite function** $f \circ g$ (also called the **composition** of $f$ and $g$) is defined by

$$
(f \circ g)(x) = f(g(x))
$$

!> In general, $f \circ g \neq g \circ f$.
</div>
